6110

Lec17/sumarray/sumarr_fill.dfy
@@ -1,8 +1,8 @@
 // Sum an array a[0]..a[a.Length-1]
 
-function recsum(a: array?<int>,Max:nat) : int // sum [0..Max)
+function recsum(a: array<int>,Max:nat) : int // sum [0..Max)
 reads a
-requires a != null
+//requires a != null
 requires 0 <= Max <= a.Length
 decreases Max
 { if a.Length == 0 then 0
@@ -10,16 +10,18 @@ decreases Max
   else a[Max-1]+recsum(a,Max-1)
 }
 
-method sumarr(a: array?<int>) returns (sum:int)
- requires a != null
+method sumarr(a: array<int>) returns (sum:int)
+ //requires a != null
  ensures sum == recsum(a,a.Length) //sum [0..a.Length)
  {sum := 0;
   if (a.Length==0) {return;}
   var i : int := 0;
   while (i < a.Length)
-  invariant ...
-  invariant ...
+  //invariant 0 <= i
+  invariant  i <= a.Length
+  invariant sum == recsum(a, i)
   {
-   sum := sum + a[i]; i:=i+1;
+   sum := sum + a[i]; 
+   i:=i+1;
   }
 }
